Lean/Geo/KGon/Var.lean
@@ -1,6 +1,7 @@
 import Mathlib.Data.Fin.Basic
 import Mathlib.Data.Prod.Lex
 import Mathlib.Data.Sum.Order
+import Geo.Definitions.Orientations
 
 /-! The CNF that we produce, as a `PropFun`. -/
 
@@ -10,23 +11,32 @@ inductive Var (n : Nat) where
   | sigma  (a b c : Fin n)
   | inside (x a b c : Fin n)
   | hole₀  (a : Fin (n+1)) (b c : Fin n)
-  | cap    (a c d : Fin n)
-  | cup    (a c d : Fin n)
+  | arc    (o : Orientation) (sz : Nat) (a c d : Fin n)
   | capF   (a d e : Fin n)
   deriving DecidableEq
 
 instance : Inhabited (Var (n+1)) := ⟨.sigma 0 0 0⟩
 
 def Var.hole (a b c : Fin n) := Var.hole₀ a.succ b c
+@[match_pattern] def Var.cap (a b c : Fin n) := Var.arc .cw 1 a b c
+@[match_pattern] def Var.cup (a b c : Fin n) := Var.arc .ccw 1 a b c
 
 instance : Repr (Var n) where
   reprPrec
   | .sigma a b c, _ => f!"σ {a.succ} {b.succ} {c.succ}"
   | .inside x a b c, _ => f!"inside {x.succ} {a.succ} {b.succ} {c.succ}"
   | .hole₀ a b c, _ => f!"hole {a} {b.succ} {c.succ}"
-  | .cap a b c, _ => f!"cap {a.succ} {b.succ} {c.succ}"
-  | .cup a b c, _ => f!"cup {a.succ} {b.succ} {c.succ}"
+  | .arc o sz a b c, _ => f!"arc {repr o} {sz} {a.succ} {b.succ} {c.succ}"
   | .capF a b c, _ => f!"capF {a.succ} {b.succ} {c.succ}"
+
+instance : LinearOrder Orientation :=
+  LinearOrder.lift'
+    (β := Nat)
+    (fun
+      | .cw => 0
+      | .collinear => 1
+      | .ccw => 2)
+    (by rintro ⟨⟩ ⟨⟩ <;> simp)
 
 -- TODO: make a deriving instance for `LinearOrder`
 instance : LinearOrder (Var n) :=
@@ -34,22 +44,21 @@ instance : LinearOrder (Var n) :=
     (β := (Fin n ×ₗ Fin n ×ₗ Fin n ⊕ₗ
            Fin n ×ₗ Fin n ×ₗ Fin n ×ₗ Fin n ⊕ₗ
            Fin (n+1) ×ₗ Fin n ×ₗ Fin n) ⊕ₗ
-           Fin n ×ₗ Fin n ×ₗ Fin n ⊕ₗ
-           Fin n ×ₗ Fin n ×ₗ Fin n ⊕ₗ
+           Orientation ×ₗ Nat ×ₗ Fin n ×ₗ Fin n ×ₗ Fin n ⊕ₗ
            Fin n ×ₗ Fin n ×ₗ Fin n)
     (fun
       | .sigma a b c => .inlₗ <| .inlₗ (a, b, c)
       | .inside x a b c => .inlₗ <| .inrₗ <| .inlₗ (x, a, b, c)
       | .hole₀ a b c => .inlₗ <| .inrₗ <| .inrₗ (a, b, c)
-      | .cap a c d => .inrₗ <| .inlₗ (a, c, d)
-      | .capF a d e => .inrₗ <| .inrₗ <| .inlₗ (a, d, e)
-      | .cup a c d => .inrₗ <| .inrₗ <| .inrₗ (a, c, d))
+      | .arc o sz a c d => .inrₗ <| .inlₗ (o, sz, a, c, d)
+      | .capF a d e => .inrₗ <| .inrₗ (a, d, e))
     (by rintro ⟨⟩ ⟨⟩ <;> simp <;> rintro ⟨⟩ <;> simp)
 
 def Var.toCode : Var n → String
   | .sigma a b c => s!"0 0 {a} {b} {c}"
   | .inside x a b c => s!"1 {x} {a} {b} {c}"
   | .hole₀ a b c => s!"2 0 {a} {b} {c}"
-  | .cap a b c => s!"3 0 {a} {b} {c}"
-  | .cup a b c => s!"4 0 {a} {b} {c}"
+  | .arc .cw sz a b c => s!"3 {sz} {a} {b} {c}"
+  | .arc .ccw sz a b c => s!"4 {sz} {a} {b} {c}"
   | .capF a b c => s!"5 0 {a} {b} {c}"
+  | .arc .collinear .. => s!"!"
